implemented trivial reflection example

coq/lc_instrumentation.v
@@ -110,13 +110,12 @@ Fixpoint replace {A:Type} (n:nat) (x:A) (l:list A) : list A :=
     end
   end.
 
+Definition config : Type := tm * store.
 
 Reserved Notation "t1 '/' st1 '-->' t2 '/' st2"
   (at level 40, st1 at level 39, t2 at level 39).
 
-Import ListNotations.
-
-Inductive step : tm * store -> tm * store -> Prop :=
+Inductive step : config -> config -> Prop :=
   | ST_AppAbs : forall x t12 v2 st,
          value v2 ->
          app (abs x t12) v2 / st --> [x:=v2]t12 / st
@@ -186,7 +185,7 @@ Notation "t1 '/' st '-->*' t2 '/' st'" :=
                (at level 40, st at level 39, t2 at level 39).
 
 
-Fixpoint stepfn (t : tm) (s : store) : tm * store :=
+Fixpoint stepfn' (t : tm) (s : store) : config :=
   match t with
   | var _ | unit | const _ | abs _ _ | loc _ | error _ => (t,s)
   | app fn arg =>
@@ -197,10 +196,10 @@ Fixpoint stepfn (t : tm) (s : store) : tm * store :=
         | _ => (error "attempt to apply non-fn", s)
         end
       else
-        let (arg',s') := stepfn arg s in
+        let (arg',s') := stepfn' arg s in
         (app fn arg', s')
     else
-      let (fn',s') := stepfn fn s in
+      let (fn',s') := stepfn' fn s in
       (app fn' arg, s')
   | scc t1 =>
     if (valueb t1) then
@@ -209,7 +208,7 @@ Fixpoint stepfn (t : tm) (s : store) : tm * store :=
       | _ => (error "scc of non nat", s)
       end
     else
-      let (t1', s') := stepfn t1 s in
+      let (t1', s') := stepfn' t1 s in
       (scc t1', s')
   | prd t1 =>
     if (valueb t1) then
@@ -218,7 +217,7 @@ Fixpoint stepfn (t : tm) (s : store) : tm * store :=
       | _ => (error "prd of non nat", s)
       end
     else
-      let (t1', s') := stepfn t1 s in
+      let (t1', s') := stepfn' t1 s in
       (prd t1', s')
   | test0 cond yes no =>
     if (valueb cond) then
@@ -228,13 +227,13 @@ Fixpoint stepfn (t : tm) (s : store) : tm * store :=
       | _ => (error "test0 of non nat", s)
       end
     else
-      let (cond', s') := stepfn cond s in
+      let (cond', s') := stepfn' cond s in
       (test0 cond' yes no, s')
   | ref t1 =>
     if (valueb t1) then
       (loc (length s), (s ++ t1::nil))
     else
-      let (t1', s') := stepfn t1 s in
+      let (t1', s') := stepfn' t1 s in
       (ref t1', s')
   | deref t1 =>
     if (valueb t1) then
@@ -246,7 +245,7 @@ Fixpoint stepfn (t : tm) (s : store) : tm * store :=
       | _ => (error "attempt to deref non-loc", s)
       end
     else
-      let (t1', s') := stepfn t1 s in
+      let (t1', s') := stepfn' t1 s in
       (deref t1', s')
   | assign t1 t2 =>
     if (valueb t1) then
@@ -259,13 +258,17 @@ Fixpoint stepfn (t : tm) (s : store) : tm * store :=
         | _ => (error "attempt to assign non-loc", s)
         end
       else
-        let (t2', s') := stepfn t2 s in
+        let (t2', s') := stepfn' t2 s in
         (assign t1 t2', s')
     else
-      let (t1', s') := stepfn t1 s in
+      let (t1', s') := stepfn' t1 s in
       (assign t1' t2, s')   
   end.
+Hint Unfold stepfn'.
 
+Definition stepfn (c : config) : config :=
+  let (t, s) := c in stepfn' t s.
+Hint Unfold stepfn.
 
 Lemma step_not_value : forall t s t' s',
     t / s --> t' / s' -> ~(value t).
@@ -310,683 +313,53 @@ Ltac stepfn_sound_tac4 :=
     specialize (H s t' s' H1); now rewrite H
   | [ H : (forall _ _ _, (?t / _ --> _ / _) -> _) |- _ ] => auto
   end.
-                                     
+
+
+                                       
 Ltac stepfn_sound_tac :=
   stepfn_sound_tac1; stepfn_sound_tac2;
   try stepfn_sound_tac3; try stepfn_sound_tac4.
 
 Theorem stepfn_sound : forall t1 s1 t2 s2,
-    t1 / s1 --> t2 / s2 -> stepfn t1 s1 = (t2, s2).
+    t1 / s1 --> t2 / s2 -> stepfn (t1, s1) = (t2, s2).
 Proof.
-  intros t1.
-  induction t1; intros; inversion H; subst; simpl; stepfn_sound_tac.
+  induction t1; intros; inversion H; subst; simpl; unfold stepfn in *; stepfn_sound_tac.
   - apply Nat.ltb_lt in H1. now rewrite H1.
   - apply Nat.ltb_lt in H6. now rewrite H6.
 Qed.
 
 
+(* META LANGUAGE *)
 
-(* --------------------------------------------------- *)
-(* META LANGUAGE - add counters to stores, incremented each time
-   the loc is refed, derefed, or assigned *)
+(* trivial example: just count the number of steps *)
+Definition metainfo : Type := nat.
 
+Definition metaconfig : Type := config * metainfo.
 
-Inductive mtm : Type :=
-  | mvar    : string -> mtm
-  | mapp    : mtm -> mtm -> mtm
-  | mabs    : string -> mtm -> mtm
-  | mconst  : nat -> mtm
-  | mscc    : mtm -> mtm
-  | mprd    : mtm -> mtm
-  | mtest0  : mtm -> mtm -> mtm -> mtm
-  | munit   : mtm
-  | mref    : mtm -> mtm
-  | mderef  : mtm -> mtm
-  | massign : mtm -> mtm -> mtm
-  | mloc    : nat -> mtm
-  | merror  : string -> mtm.
+Definition reify (c : config) : metaconfig := (c, 0).
 
-(* values *)
-Inductive mvalue : mtm -> Prop :=
-  | mv_abs  : forall x t,
-      mvalue (mabs x t)
-  | mv_nat : forall n,
-      mvalue (mconst n)
-  | mv_unit :
-      mvalue munit
-  | mv_loc : forall l,
-      mvalue (mloc l).
-Hint Constructors mvalue.
+Definition reflect (mc : metaconfig) : config :=
+  let (c, _) := mc in c.
 
-Fixpoint mvalueb (mt : mtm) : bool :=
-  match mt with
-  | mabs _ _ | mconst _ | munit | mloc _ => true
-  | _ => false
-  end.
+Definition infostepfn (mc : metaconfig) : metainfo :=
+  let (_, n) := mc in S n.
 
-Theorem mvalueb_sound : forall mt, mvalue mt -> (mvalueb mt = true).
-Proof.
-  intros.
-  inversion H; simpl; reflexivity.
-Qed.
+Definition configstepfn (mc : metaconfig) : config :=
+  let (c, _) := mc in stepfn c.
 
-Theorem mvalueb_complete : forall mt, (mvalueb mt = true) -> mvalue mt.
-Proof.
-  intros.
-  destruct mt; simpl; try discriminate; auto.
-Qed.
-
-(* substitution. NB ignores free-variable issues. *)
-Fixpoint msubst (x:string) (s:mtm) (t:mtm) : mtm :=
-  match t with
-  | mvar x'       =>
-      if String.eqb x x' then s else t
-  | mapp t1 t2    =>
-      mapp (msubst x s t1) (msubst x s t2)
-  | mabs x' t1  =>
-      if String.eqb x x' then t else mabs x' (msubst x s t1)
-  | mconst n        =>
-      t
-  | mscc t1      =>
-      mscc (msubst x s t1)
-  | mprd t1      =>
-      mprd (msubst x s t1)
-  | mtest0 t1 t2 t3 =>
-      mtest0 (msubst x s t1) (msubst x s t2) (msubst x s t3)
-  | munit         =>
-      t
-  | mref t1       =>
-      mref (msubst x s t1)
-  | mderef t1     =>
-      mderef (msubst x s t1)
-  | massign t1 t2 =>
-      massign (msubst x s t1) (msubst x s t2)
-  | mloc _        =>
-      t
-  | merror _      => t 
-  end.
-
-
-Definition mstore := list (mtm * nat).
-
-Definition mstore_lookup (n:nat) (mst:mstore) :=
-  match nth n mst (munit, O) with
-  | (mt, _) => mt
-  end.
-
-Definition mstore_incr_loc (n:nat) (mst:mstore) :=
-  match nth n mst (munit, O) with
-  | (mt, ct) => replace n (mt, S ct) mst
-  end. 
-
-Definition replace_incr_loc (n:nat) (t:mtm) (mst:mstore) :=
-  match nth n mst (munit, O) with
-  | (_, ct) => replace n (t, S ct) mst
-  end. 
-
-Reserved Notation "t1 '/' st1 '-m>' t2 '/' st2"
-  (at level 40, st1 at level 39, t2 at level 39).
-
-Inductive metastep : mtm * mstore -> mtm * mstore -> Prop :=
-  | MST_AppAbs : forall x t12 v2 st,
-         mvalue v2 ->
-         mapp (mabs x t12) v2 / st -m> msubst x v2 t12 / st
-  | MST_App1 : forall t1 t1' t2 st st',
-         t1 / st -m> t1' / st' ->
-         mapp t1 t2 / st -m> mapp t1' t2 / st'
-  | MST_App2 : forall v1 t2 t2' st st',
-         mvalue v1 ->
-         t2 / st -m> t2' / st' ->
-         mapp v1 t2 / st -m> mapp v1 t2'/ st'
-  | MST_SuccNat : forall n st,
-         mscc (mconst n) / st -m> mconst (S n) / st
-  | MST_Succ : forall t1 t1' st st',
-         t1 / st -m> t1' / st' ->
-         mscc t1 / st -m> mscc t1' / st'
-  | MST_PredNat : forall n st,
-         mprd (mconst n) / st -m> mconst (pred n) / st
-  | MST_Pred : forall t1 t1' st st',
-         t1 / st -m> t1' / st' ->
-         mprd t1 / st -m> mprd t1' / st'
-  | MST_If0 : forall t1 t1' t2 t3 st st',
-         t1 / st -m> t1' / st' ->
-         mtest0 t1 t2 t3 / st -m> mtest0 t1' t2 t3 / st'
-  | MST_If0_Zero : forall t2 t3 st,
-         mtest0 (mconst 0) t2 t3 / st -m> t2 / st
-  | MST_If0_Nonzero : forall n t2 t3 st,
-         mtest0 (mconst (S n)) t2 t3 / st -m> t3 / st
-  | MST_Refvalue : forall v1 st,
-         mvalue v1 ->
-         mref v1 / st -m> mloc (length st) / (st ++ (v1,0)::nil)
-  | MST_Ref : forall t1 t1' st st',
-         t1 / st -m> t1' / st' ->
-         mref t1 /  st -m> mref t1' /  st'
-  | MST_DerefLoc : forall st l,
-         l < length st ->
-         mderef (mloc l) / st -m> mstore_lookup l st / mstore_incr_loc l st
-  | MST_Deref : forall t1 t1' st st',
-         t1 / st -m> t1' / st' ->
-         mderef t1 / st -m> mderef t1' / st'
-  | MST_Assign : forall v2 l st,
-         mvalue v2 ->
-         l < length st ->
-         massign (mloc l) v2 / st -m> munit / replace_incr_loc l v2 st
-  | MST_Assign1 : forall t1 t1' t2 st st',
-         t1 / st -m> t1' / st' ->
-         massign t1 t2 / st -m> massign t1' t2 / st'
-  | MST_Assign2 : forall v1 t2 t2' st st',
-         mvalue v1 ->
-         t2 / st -m> t2' / st' ->
-         massign v1 t2 / st -m> massign v1 t2' / st'
-where "t1 '/' st1 '-m>' t2 '/' st2" := (metastep (t1,st1) (t2,st2)).
-Hint Constructors metastep.
-
-Fixpoint mstepfn (t : mtm) (s : mstore) : mtm * mstore :=
-  match t with
-  | mvar _ | munit | mconst _ | mabs _ _ | mloc _ | merror _ => (t,s)
-  | mapp fn arg =>
-    if (mvalueb fn) then
-      if (mvalueb arg) then
-        match fn with
-        | mabs x body => (msubst x arg body, s)
-        | _ => (merror "attempt to apply non-fn", s)
-        end
-      else
-        let (arg',s') := mstepfn arg s in
-        (mapp fn arg', s')
-    else
-      let (fn',s') := mstepfn fn s in
-      (mapp fn' arg, s')
-  | mscc t1 =>
-    if (mvalueb t1) then
-      match t1 with
-      | mconst n => (mconst (S n), s)
-      | _ => (merror "scc of non nat", s)
-      end
-    else
-      let (t1', s') := mstepfn t1 s in
-      (mscc t1', s')
-  | mprd t1 =>
-    if (mvalueb t1) then
-      match t1 with
-      | mconst n => (mconst (pred n), s)
-      | _ => (merror "prd of non nat", s)
-      end
-    else
-      let (t1', s') := mstepfn t1 s in
-      (mprd t1', s')
-  | mtest0 cond yes no =>
-    if (mvalueb cond) then
-      match cond with
-      | mconst 0 => (yes, s)
-      | mconst (S n) => (no, s)
-      | _ => (merror "test0 of non nat", s)
-      end
-    else
-      let (cond', s') := mstepfn cond s in
-      (mtest0 cond' yes no, s')
-  (* Add instrumentation to the store *)
-  | mref t1 =>
-    if (mvalueb t1) then
-      (mloc (length s), (s ++ (t1,0)::nil))
-    else
-      let (t1', s') := mstepfn t1 s in
-      (mref t1', s')
-  | mderef t1 =>
-    if (mvalueb t1) then
-      match t1 with
-      | mloc l =>
-        if Nat.ltb l (length s) then
-          (mstore_lookup l s, mstore_incr_loc l s)
-        else (merror "attempt to deref invalid loc", s)
-      | _ => (merror "attempt to deref non-loc", s)
-      end
-    else
-      let (t1', s') := mstepfn t1 s in
-      (mderef t1', s')
-  | massign t1 t2 =>
-    if (mvalueb t1) then
-      if (mvalueb t2) then
-        match t1 with
-        | mloc l =>
-          if Nat.ltb l (length s) then
-            (munit, replace_incr_loc l t2 s)
-          else (merror "attempt to assign invalid loc", s)
-        | _ => (merror "attempt to assign non-loc", s)
-        end
-      else
-        let (t2', s') := mstepfn t2 s in
-        (massign t1 t2', s')
-    else
-      let (t1', s') := mstepfn t1 s in
-      (massign t1' t2, s')   
-  end.
-
-Theorem mstepfn_sound :
-  forall mt ms mt' ms',
-    mt / ms -m> mt' / ms' ->
-    mstepfn mt ms = (mt', ms').
-Proof.
-  intros mt; induction mt; intros; subst; simpl; inversion H; admit.
-  (* todo - same as stepfn_sound *)
-Admitted.
-
-Inductive reify_tm : tm -> mtm -> Prop :=
-| Reify_Var :
-    forall x, reify_tm (var x) (mvar x)
-| Reify_App :
-    forall t1 t2 mt1 mt2,
-      reify_tm t1 mt1 -> reify_tm t2 mt2 ->
-      reify_tm (app t1 t2) (mapp mt1 mt2)
-| Reify_Abs :
-    forall x t1 mt1,
-      reify_tm t1 mt1 ->
-      reify_tm (abs x t1) (mabs x mt1)
-| Reify_Const :
-    forall n, reify_tm (const n) (mconst n)
-| Reify_Scc :
-    forall t1 mt1,
-      reify_tm t1 mt1 ->
-      reify_tm (scc t1) (mscc mt1)
-| Reify_Prd :
-    forall t1 mt1,
-      reify_tm t1 mt1 ->
-      reify_tm (prd t1) (mprd mt1)    
-| Reify_Test0 :
-    forall t1 t2 t3 mt1 mt2 mt3,
-      reify_tm t1 mt1 ->
-      reify_tm t2 mt2 ->
-      reify_tm t3 mt3 ->
-      reify_tm (test0 t1 t2 t3) (mtest0 mt1 mt2 mt3)
-| Reify_Unit :
-    reify_tm unit munit
-| Reify_Ref :
-    forall t1 mt1,
-      reify_tm t1 mt1 ->
-      reify_tm (ref t1) (mref mt1)
-| Reify_Deref :
-    forall t1 mt1,
-      reify_tm t1 mt1 ->
-      reify_tm (deref t1) (mderef mt1)
-| Reify_Assign :
-    forall t1 t2 mt1 mt2,
-      reify_tm t1 mt1 ->
-      reify_tm t2 mt2 ->
-      reify_tm (assign t1 t2) (massign mt1 mt2)
-| Reify_Loc :
-    forall l, reify_tm (loc l) (mloc l)
-| Reify_Error :
-    forall s, reify_tm (error s) (merror s).
-Hint Constructors reify_tm.
-
-Fixpoint reify_tm_fn (t : tm) : mtm :=
-  match t with
-  | var x' => mvar x'
-  | app t1 t2 => mapp (reify_tm_fn t1) (reify_tm_fn t2)
-  | abs x' t1 => mabs x' (reify_tm_fn t1)
-  | const n => mconst n
-  | scc t1 => mscc (reify_tm_fn t1)
-  | prd t1 => mprd (reify_tm_fn t1)
-  | test0 t1 t2 t3 => mtest0 (reify_tm_fn t1) (reify_tm_fn t2) (reify_tm_fn t3)
-  | unit => munit
-  | ref t1 => mref (reify_tm_fn t1)
-  | deref t1  => mderef (reify_tm_fn t1)
-  | assign t1 t2 => massign (reify_tm_fn t1) (reify_tm_fn t2)
-  | loc l => mloc l
-  | error s => merror s 
-  end.
-
-Theorem reify_tm_fn_sound :
-  forall t mt,
-    reify_tm t mt -> reify_tm_fn t = mt.
-Proof.
-  (* how to automate this proof?? it's pretty boilerplate-y *)
-  intros t; induction t; intros; cbn; inversion H; subst; try reflexivity;
-    try (specialize (IHt mt1); specialize (IHt H1); rewrite -> IHt; reflexivity).
-  - specialize (IHt1 mt1). specialize (IHt1 H2). rewrite -> IHt1.
-    specialize (IHt2 mt2). specialize (IHt2 H4). rewrite -> IHt2.
-    reflexivity.
-  - specialize (IHt mt1).  specialize (IHt H3).  rewrite -> IHt.
-    reflexivity.
-  - specialize (IHt1 mt1). specialize (IHt1 H3). rewrite -> IHt1.
-    specialize (IHt2 mt2). specialize (IHt2 H5). rewrite -> IHt2.
-    specialize (IHt3 mt3). specialize (IHt3 H6). rewrite -> IHt3.
-    reflexivity.
-  - specialize (IHt1 mt1). specialize (IHt1 H2). rewrite -> IHt1.
-    specialize (IHt2 mt2). specialize (IHt2 H4). rewrite -> IHt2.
-    reflexivity.
-Qed.
-
-(* think about the O here - how to make it general *)
-Inductive reify_st : store -> mstore -> Prop :=
-| ReifySt_Nil: reify_st [] []
-| ReifySt_Cons:
-    forall t mt s ms,
-      reify_st s ms ->
-      reify_tm t mt ->
-      reify_st (t::s) ((mt, O)::ms).
-Hint Constructors reify_st.
-
-Definition reify_st_fn (st : store) : mstore :=
-  map (fun t => (reify_tm_fn t, O)) st.
-
-Theorem reify_st_fn_sound :
-  forall s ms,
-    reify_st s ms -> reify_st_fn s = ms.
-Proof.
-  intros s; induction s; intros; inversion H; subst.
-  - reflexivity.
-  - simpl.
-    apply reify_tm_fn_sound in H4.
-    specialize (IHs ms0).
-    specialize (IHs H2).
-    rewrite -> H4.
-    rewrite -> IHs.
-    reflexivity.
-Qed.
-
-Inductive reify : tm * store -> mtm * mstore -> Prop :=
-| Reify : forall t s mt ms,
-    reify_tm t mt ->
-    reify_st s ms ->
-    reify (t, s) (mt, ms).
-Hint Constructors reify.
-
-Definition reify_fn (t : tm) (st : store) : (mtm * mstore) :=
-  (reify_tm_fn t, reify_st_fn st).
-Hint Unfold reify_fn.
-
-Theorem reify_fn_sound :
-  forall t s mt ms mt' ms',
-    reify (t, s) (mt, ms) -> reify_fn t s = (mt', ms') -> mt = mt' /\ ms = ms'.
-Proof.
-  intros.
-  inversion H; subst.
-  apply reify_tm_fn_sound in H4.
-  apply reify_st_fn_sound in H6.
-  inversion H0.
-  split.
-  - rewrite -> H4. reflexivity.
-  - rewrite -> H6. reflexivity.
-Qed.
-
-Inductive reflect_mtm : mtm -> tm -> Prop :=
-| Reflect_Var :
-    forall x, reflect_mtm (mvar x) (var x)
-| Reflect_App :
-    forall mt1 mt2 t1 t2,
-      reflect_mtm mt1 t1 -> reflect_mtm mt2 t2 ->
-      reflect_mtm (mapp mt1 mt2) (app t1 t2)
-| Reflect_Abs :
-    forall x mt1 t1,
-      reflect_mtm mt1 t1 ->
-      reflect_mtm (mabs x mt1) (abs x t1)
-| Reflect_Const :
-    forall n, reflect_mtm (mconst n) (const n)
-| Reflect_Scc :
-    forall mt1 t1,
-      reflect_mtm mt1 t1 ->
-      reflect_mtm (mscc mt1) (scc t1)
-| Reflect_Prd :
-    forall t1 mt1,
-      reflect_mtm mt1 t1 ->
-      reflect_mtm (mprd mt1) (prd t1)    
-| Reflect_Test0 :
-    forall mt1 mt2 mt3 t1 t2 t3,
-      reflect_mtm mt1 t1 ->
-      reflect_mtm mt2 t2 ->
-      reflect_mtm mt3 t3 ->
-      reflect_mtm (mtest0 mt1 mt2 mt3) (test0 t1 t2 t3)
-| Reflect_Unit :
-    reflect_mtm munit unit
-| Reflect_Ref :
-    forall mt1 t1,
-      reflect_mtm mt1 t1 ->
-      reflect_mtm (mref mt1) (ref t1)
-| Reflect_Deref :
-    forall mt1 t1,
-      reflect_mtm mt1 t1 ->
-      reflect_mtm (mderef mt1) (deref t1)
-| Reflect_Assign :
-    forall mt1 mt2 t1 t2,
-      reflect_mtm mt1 t1 ->
-      reflect_mtm mt2 t2 ->
-      reflect_mtm (massign mt1 mt2) (assign t1 t2)
-| Reflect_Loc :
-    forall l, reflect_mtm (mloc l) (loc l)
-| Reflect_Error :
-    forall s, reflect_mtm (merror s) (error s).
-Hint Constructors reflect_mtm.
-
-Fixpoint reflect_mtm_fn (mt : mtm) : tm :=
-  match mt with
-  | mvar x' => var x'
-  | mapp t1 t2 => app (reflect_mtm_fn t1) (reflect_mtm_fn t2)
-  | mabs x' t1 => abs x' (reflect_mtm_fn t1)
-  | mconst n => const n
-  | mscc t1 => scc (reflect_mtm_fn t1)
-  | mprd t1 => prd (reflect_mtm_fn t1)
-  | mtest0 t1 t2 t3 => test0 (reflect_mtm_fn t1) (reflect_mtm_fn t2) (reflect_mtm_fn t3)
-  | munit => unit
-  | mref t1 => ref (reflect_mtm_fn t1)
-  | mderef t1 => deref (reflect_mtm_fn t1)
-  | massign t1 t2 => assign (reflect_mtm_fn t1) (reflect_mtm_fn t2)
-  | mloc l => loc l
-  | merror s => error s 
-  end.
-
-Theorem reflect_mtm_fn_sound :
-  forall mt t,
-    reflect_mtm mt t -> reflect_mtm_fn mt = t.
-Proof.
-  (* how to automate this proof?? it's pretty boilerplate-y *)
-  intros mt; induction mt; intros; cbn; inversion H; subst; try reflexivity;
-    try (specialize (IHmt t1); specialize (IHmt H1); rewrite -> IHmt; reflexivity).
-  - specialize (IHmt1 t1). specialize (IHmt1 H2). rewrite -> IHmt1.
-    specialize (IHmt2 t2). specialize (IHmt2 H4). rewrite -> IHmt2.
-    reflexivity.
-  - specialize (IHmt t1).  specialize (IHmt H3).  rewrite -> IHmt.
-    reflexivity.
-  - specialize (IHmt1 t1). specialize (IHmt1 H3). rewrite -> IHmt1.
-    specialize (IHmt2 t2). specialize (IHmt2 H5). rewrite -> IHmt2.
-    specialize (IHmt3 t3). specialize (IHmt3 H6). rewrite -> IHmt3.
-    reflexivity.
-  - specialize (IHmt1 t1). specialize (IHmt1 H2). rewrite -> IHmt1.
-    specialize (IHmt2 t2). specialize (IHmt2 H4). rewrite -> IHmt2.
-    reflexivity.
-Qed.
-
-Inductive reflect_mst : mstore -> store -> Prop :=
-| ReflectMst_Nil: reflect_mst [] []
-| ReflectMst_Cons:
-    forall mt t ms s n,
-      reflect_mst ms s ->
-      reflect_mtm mt t ->
-      reflect_mst ((mt, n)::ms) (t::s).
-Hint Constructors reflect_mst.
-
-Definition reflect_mst_fn (mst : mstore) : store :=
-  map (fun pair =>
-         match pair with
-         | (t, _) => reflect_mtm_fn t
-         end)
-      mst.
-
-Theorem reflect_mst_fn_sound :
-  forall ms s,
-    reflect_mst ms s -> reflect_mst_fn ms = s.
-Proof.
-  intros s; induction s; intros; inversion H; subst.
-  - auto.
-  - simpl.
-    apply reflect_mtm_fn_sound in H4.
-    specialize (IHs s1).
-    specialize (IHs H2).
-    rewrite -> H4.
-    rewrite -> IHs.
-    reflexivity.
-Qed.
-
-Inductive reflect : mtm * mstore -> tm * store -> Prop :=
-| Reflect :
-    forall mt ms t s,
-      reflect_mtm mt t ->
-      reflect_mst ms s ->
-      reflect (mt, ms) (t, s).
-Hint Constructors reflect.
-
-Definition reflect_fn (mt : mtm) (mst : mstore) : (tm * store) :=
-  (reflect_mtm_fn mt, reflect_mst_fn mst).
-
-Theorem reflect_fn_sound :
-  forall mt ms t s t' s',
-    reflect (mt, ms) (t, s) ->
-    reflect_fn mt ms = (t', s') ->
-    t = t' /\ s = s'.
-Proof.
-  intros.
-  inversion H; subst.
-  apply reflect_mtm_fn_sound in H4.
-  apply reflect_mst_fn_sound in H6.
-  inversion H0.
-  split.
-  - rewrite -> H4. reflexivity.
-  - rewrite -> H6. reflexivity.
-Qed.
-
-Lemma reify_reflect_inv_t :
-  forall t s mt ms ms' t' s',
-    reify (t, s) (mt, ms) ->
-    reflect (mt, ms') (t', s') ->
-    t = t'.
-Proof.
-  intros t; induction t; intros;
-  inversion H ; subst; inversion H0; subst; inversion H4; subst;
-  inversion H5; subst; inversion H6; subst; inversion H8; subst;
-    eauto;
-    try (assert (t = t1) as TT1 by eauto;
-         rewrite TT1; reflexivity);
-    try (assert (t1 = t0) as T1T0 by eauto;
-         assert (t2 = t3) as T2T3 by eauto;
-         rewrite T1T0; rewrite T2T3; reflexivity);
-    try (assert (t1 = t0) as T1T0 by eauto;
-         assert (t2 = t4) as T2T4 by eauto;
-         assert (t3 = t5) as T3T5 by eauto;
-         rewrite T1T0; rewrite T2T4; rewrite T3T5; reflexivity).
-Qed.
-
-Lemma reify_st_reflect_mst_inv :
-  forall s ms s',
-    reify_st s ms ->
-    reflect_mst ms s' ->
-    s = s'.
-Proof.
-  intros s; induction s; intros.
-  inversion H; subst; inversion H0; subst; auto.
-  inversion H; subst. inversion H0; subst.
-  assert (a = t) by eauto using reify_reflect_inv_t. rewrite H1.
-  specialize (IHs ms0 s0 H3 H7). rewrite IHs.
-  auto.
-Qed.
-
-Lemma reify_reflect_inv_s :
-  forall t s mt mt' ms t' s',
-    reify (t, s) (mt, ms) ->
-    reflect (mt', ms) (t', s') ->
-    s = s'.
-Proof.
-  intros.
-  inversion H; subst; inversion H0; subst.
-  generalize H8. generalize H6.
-  apply reify_st_reflect_mst_inv.
-Qed.
-
-Lemma reify_reflect_inv :
-  forall t s mt ms t' s',
-    reify (t, s) (mt, ms) ->
-    reflect (mt, ms) (t', s') ->
-    t = t' /\ s = s'.
-Proof.
-  intros. split.
-  - eauto using reify_reflect_inv_t.
-  - eauto using reify_reflect_inv_s.
-Qed.
-
-Ltac invsubst x := inversion x; subst.
-
-Ltac pinvsubst x := idtac x; invsubst x.
-
-Ltac invert_something :=
-  match goal with
-  | [ H : metastep _ _ |- _] => pinvsubst H
-  | [ H : reify _ _ |- _] => pinvsubst H
-  | [ H : reflect _ _ |- _] => pinvsubst H
-  | [ H : reify_tm _ _ |- _] => pinvsubst H
-  | [ H : reify_st _ _ |- _] => pinvsubst H
-  | [ H : reflect_mtm _ _ |- _] => pinvsubst H
-  | [ H : reflect_mst _ _ |- _] => pinvsubst H
-  | _ => idtac
-  end.
-
-Ltac invert_all := repeat (try (progress invert_something)).
-
-Lemma reify_preserves_values :
-  forall t mt,
-    reify_tm t mt ->
-    value t -> mvalue mt.
-Proof.
-  intros t mt R V; invsubst V; invsubst R; eauto.
-Qed.
-
-Lemma reify_preserves_mvalues :
-  forall t mt,
-    reify_tm t mt -> mvalue mt -> value t.
-Proof.
-  - intros t mt R MV; invsubst MV; invsubst R; eauto.
-Qed.
-
-Lemma mvalue_not_metastep :
-  forall mt ms,
-    mvalue mt ->
-    ~ (exists mt' ms', mt / ms -m> mt' / ms').
-Proof.
-  intros; inversion H; intuition; inversion H1; inversion H2; inversion H3.
-Qed.
+Definition metastepfn (mc : metaconfig) : metaconfig :=
+  (configstepfn mc, infostepfn mc).
 
 Theorem reflection_sound :
-  forall t s t' s' mt ms mt' ms' t'' s'',
-    t / s --> t' / s' ->
-    reify (t, s) (mt, ms) ->
-    mt / ms -m> mt' / ms' ->
-    reflect (mt', ms') (t'', s'') ->
-    t' = t'' /\ s' = s''.
+  forall c c',
+    step c c' ->
+    reflect (metastepfn (reify c)) = c'.
 Proof.
-  intros t.
-  induction t; intros; invsubst H; simpl.
-  - invsubst H0. invsubst H7. invsubst H6.
-    assert (mvalue mt2) by eauto using reify_preserves_values.
-    assert (mvalue (mabs x mt0)) by eauto.
-    invsubst H1.
-    + admit.
-    + invsubst H12.
-    + exfalso. specialize (mvalue_not_metastep mt2 ms H3). intuition.
-      apply H8. exists t2'. exists ms'. exact H17.
-  - admit.
-  - admit.
-  - invsubst H0. invsubst H6. invsubst H1.
-    + invsubst H2. invsubst H9. invsubst H4. intuition.
-      eapply reify_reflect_inv_s; eauto.
-    + invsubst H0. invsubst H10. invsubst H9.
-      invsubst H5.
-  - invsubst H0.
-    invsubst H7.
-    assert (~value t) by eauto using step_not_value.
-    assert (~ mvalue mt1) by eauto using reify_preserves_mvalues.
-    
-    specialize (IHt s t1' s' ).
-    assert (reify (t, s) (mt1, ms)) by eauto.    
-    
-    
-       
+  intros; cbn; destruct c; destruct c'; eauto using stepfn_sound.
+Qed.
+
+
+
+
 
 
